theories/FOL/minZF.v
@@ -1,0 +1,155 @@
+(** * Definition of semantic and deductive ZF-Entailment in minimal signature *)
+
+Require Import Undecidability.FOL.Util.Syntax.
+Require Import Undecidability.FOL.Util.FullTarski.
+Require Import Undecidability.FOL.Util.FullDeduction.
+Require Import Undecidability.FOL.ZF.
+Require Import List.
+
+
+ 
+(** ** Minimal signature *)
+
+Instance sig_empty : funcs_signature :=
+    {| syms := False;  ar_syms := False_rect nat |}.
+
+Existing Instance ZF_func_sig.
+
+Notation term' := (term sig_empty).
+Notation form' := (form sig_empty _ _ falsity_on).
+
+Definition embed_t (t : term') : term :=
+  match t with
+  | $x => $x
+  | func f ts => False_rect term f
+  end.
+
+Fixpoint embed {ff'} (phi : form sig_empty ZF_pred_sig _ ff') : form ff' :=
+  match phi with 
+  | atom P ts => atom P (Vector.map embed_t ts)
+  | bin b phi psi => bin b (embed phi) (embed psi)
+  | quant q phi => quant q (embed phi)
+  | ⊥ => ⊥
+  end.
+
+Notation "x ∈' y" := (atom sig_empty ZF_pred_sig elem (Vector.cons x (Vector.cons y Vector.nil))) (at level 35).
+Notation "x ≡' y" := (atom sig_empty ZF_pred_sig equal (Vector.cons x (Vector.cons y Vector.nil))) (at level 35).
+
+
+
+(** ** Characterisations of set operations *)
+
+Fixpoint shift `{funcs_signature} `{preds_signature} n (t : term) :=
+  match n with 
+  | O => t
+  | S n => subst_term ↑ (shift n t)
+  end.
+
+Definition is_eset (t : term') :=
+  ∀ ¬ ($0 ∈ t`[↑]).
+
+Definition is_pair (x y t : term') :=
+  ∀ $0 ∈ t`[↑] <--> $0 ≡ x`[↑] ∨ $0 ≡ y`[↑].
+
+Definition is_union (x t : term') :=
+  ∀ $0 ∈ t`[↑] <--> ∃ $0 ∈ shift 2 x ∧ $1 ∈ $0.
+
+Definition sub' (x y : term') :=
+  ∀ $0 ∈ x`[↑] --> $0 ∈ y`[↑].
+
+Definition is_power (x t : term') :=
+  ∀ $0 ∈ t`[↑] <--> sub' $0 x`[↑].
+
+Definition is_sigma (x t : term') :=
+  ∀ $0 ∈ t`[↑] <--> $0 ∈ x`[↑] ∨ $0 ≡ x`[↑].
+
+Definition is_inductive (t : term') :=
+  (∃ is_eset $0 ∧ $0 ∈ t`[↑]) ∧ ∀ $0 ∈ t`[↑] --> (∃ is_sigma $1 $0 ∧ $0 ∈ shift 2 t).
+
+Definition is_om (t : term') :=
+  is_inductive t ∧ ∀ is_inductive $0 --> sub' t`[↑] $0.
+
+
+
+(** ** Symbol-free axiomatisation *)
+
+Definition ax_ext' :=
+  ∀ ∀ sub' $1 $0 --> sub' $0 $1 --> $1 ≡' $0.
+
+Definition ax_eset' :=
+  ∃ is_eset $0.
+
+Definition ax_pair' :=
+  ∀ ∀ ∃ is_pair $2 $1 $0.
+
+Definition ax_union' :=
+  ∀ ∃ is_union $1 $0.
+
+Definition ax_power' :=
+  ∀ ∃ is_power $1 $0.
+
+Definition ax_om' :=
+  ∃ is_om $0.
+
+Definition ax_refl' :=
+  ∀ $0 ≡' $0.
+
+Definition ax_sym' :=
+  ∀ ∀ $1 ≡' $0 --> $0 ≡' $1.
+
+Definition ax_trans' :=
+  ∀ ∀ ∀ $2 ≡' $1 --> $1 ≡' $0 --> $2 ≡' $0.
+
+Definition ax_eq_elem' :=
+  ∀ ∀ ∀ ∀ $3 ≡' $1 --> $2 ≡' $0 --> $3 ∈' $2 --> $1 ∈' $0.
+
+Definition minZF' :=
+  ax_ext' :: ax_eset' :: ax_pair' :: ax_union' :: ax_power' :: ax_om' :: nil.
+
+Definition minZFeq' :=
+  ax_refl' :: ax_sym' :: ax_trans' :: ax_eq_elem' :: minZF'.
+
+Definition ax_sep' phi :=
+  ∀ ∃ ∀ $0 ∈' $1 <--> $0 ∈' $2 ∧ phi[$0.: Nat.add 3 >> var].
+
+Definition fun_rel' phi :=
+  ∀ ∀ ∀ phi[$2 .: $1 .: Nat.add 3 >> var] --> phi[$2 .: $0 .: Nat.add 3 >> var] --> $1 ≡' $0.
+
+Definition ax_rep' phi :=
+  fun_rel' phi --> ∀ ∃ ∀ $0 ∈' $1 <--> ∃ $0 ∈' $3 ∧ phi[$0 .: $1 .: Nat.add 4 >> var].
+
+Inductive minZF : form' -> Prop :=
+| minZF_base phi : In phi minZF' -> minZF phi
+| minZF_sep phi : minZF (ax_sep' phi)
+| minZF_rep phi : minZF (ax_rep' phi).
+
+Inductive minZFeq : form' -> Prop :=
+| minZFeq_base phi : In phi minZFeq' -> minZFeq phi
+| minZFeq_sep phi : minZFeq (ax_sep' phi)
+| minZFeq_rep phi : minZFeq (ax_rep' phi).
+
+
+
+(** ** Problems *)
+
+(* Semantic entailment restricted to extensional models and core axioms (without sep and rep). *)
+
+Definition entailment_minZF' phi :=
+  forall D (M : @interp sig_empty _ D) (rho : nat -> D), extensional M -> (forall sigma psi, In psi minZF' -> sigma ⊨ psi) -> rho ⊨ phi.
+
+(* Semantic entailment restricted to extensional models. *)
+
+Definition entailment_minZF phi :=
+  forall D (M : @interp sig_empty _ D) (rho : nat -> D), extensional M -> (forall sigma psi, minZF psi -> sigma ⊨ psi) -> rho ⊨ phi.
+
+(* Deductive entailment restricted to intuitionistic rules and core axioms (without sep and rep). *)
+
+Definition deduction_minZF' phi :=
+  minZFeq' ⊢I phi.
+
+(* Deductive entailment restricted to intuitionistic rules. *)
+
+Definition deduction_minZF phi :=
+  minZFeq ⊢TI phi.
+
+
